added SeqExt.map.

src/specs/seqext.fsi
@@ -24,13 +24,68 @@
 module Tesseract.Specs.SeqExt
    open Seq
 
+   val map:
+      // high-order mapping function
+      ('a -> Tot 'b)
+      // input sequence
+      -> s: seq 'a
+      // output sequence
+      -> Tot (seq 'b)
+
    val mem: seq 'a -> 'a -> Tot bool
+
+   val filter:
+      ('a -> Tot bool)
+         // predicate; if false, then the element is discarded from the
+         // sequence.
+      -> seq 'a // input sequence
+      -> Tot (seq 'a) // output sequence
+
+   val insert:
+      s: seq 'a
+      -> i: nat{i <= length s}
+      -> 'a
+      -> Tot (seq 'a)
+
+   val remove:
+      s: seq 'a{length s > 0}
+      -> i: nat{i < length s}
+      -> 'a
+      -> Tot (seq 'a)
+
+   // lemmas
+
+   val lemma_map__length:
+      f: ('a -> Tot 'b)
+      -> s: seq 'a
+      -> Lemma
+         (requires (True))
+            // bug: if the parenthesis is dropped from the preceeding
+            // expression, f* will silently fail to build the definition if
+            // included as a dependency.
+         (ensures (length (map f s) = length s))
+         [SMTPat (length (map f s))]
+
+   val lemma_map__map:
+      f: ('a -> Tot 'b)
+      -> s: seq 'a
+      -> i: nat{i < length s}
+      -> Lemma
+         (requires (True))
+            // bug: if the parenthesis is dropped from the preceeding
+            // expression, f* will silently fail to build the definition if
+            // included as a dependency.
+         (ensures (index (map f s) i = f (index s i)))
+         [SMTPat (index (map f s) i)]
 
    val lemma_mem__mem:
       s: seq 'a
       -> a: 'a
       -> Lemma
-         (requires True)
+         (requires (True))
+            // bug: if the parenthesis is dropped from the preceeding
+            // expression, f* will silently fail to build the definition if
+            // included as a dependency.
          (ensures
             ((mem s a)
                ==>
@@ -40,19 +95,25 @@ module Tesseract.Specs.SeqExt
                         (index s i = a))))
          [SMTPat (mem s a)]
 
-   val filter:
-      // predicate; if false, then the element is discarded from the sequence.
-      ('a -> Tot bool)
-      // input sequence
-      -> seq 'a
-      // output sequence
-      -> Tot (seq 'a)
+   val lemma_mem__append:
+      s0: seq 'a
+      -> s1: seq 'a
+      -> Lemma
+         (requires (True))
+            // bug: if the parenthesis is dropped from the preceeding
+            // expression, f* will silently fail to build the definition if
+            // included as a dependency.
+         (ensures (exists a. (mem s0 a || mem s1 a) <==> mem (append s0 s1) a))
+         [SMTPat (append s0 s1)]
 
    val lemma_filter__length:
-      p: ('a -> Tot bool) ->
-      s: seq 'a ->
-      Lemma
-         (requires True)
+      p: ('a -> Tot bool)
+      -> s: seq 'a
+      -> Lemma
+         (requires (True))
+            // bug: if the parenthesis is dropped from the preceeding
+            // expression, f* will silently fail to build the definition if
+            // included as a dependency.
          (ensures (length (filter p s) <= length s))
          [SMTPat (length (filter p s))]
 
@@ -61,22 +122,22 @@ module Tesseract.Specs.SeqExt
       -> s: seq 'a
       -> i: nat{i < length (filter p s)}
       -> Lemma
-         (requires True)
+         (requires (True))
+            // bug: if the parenthesis is dropped from the preceeding
+            // expression, f* will silently fail to build the definition if
+            // included as a dependency.
          (ensures (p (index (filter p s) i)))
          [SMTPat (index (filter p s) i)]
-
-   val insert:
-      s: seq 'a
-      -> i: nat{i <= length s}
-      -> 'a
-      -> Tot (seq 'a)
 
    val lemma_insert__length:
       s: seq 'a
       -> i: nat{i <= length s}
       -> a: 'a
       -> Lemma
-         (requires True)
+         (requires (True))
+            // bug: if the parenthesis is dropped from the preceeding
+            // expression, f* will silently fail to build the definition if
+            // included as a dependency.
          (ensures (length (insert s i a) = length s + 1))
          [SMTPat (length (insert s i a))]
 
@@ -85,6 +146,10 @@ module Tesseract.Specs.SeqExt
       -> i: nat{i <= length s}
       -> a: 'a
       -> Lemma
+         (requires (True))
+            // bug: if the parenthesis is dropped from the preceeding
+            // expression, f* will silently fail to build the definition if
+            // included as a dependency.
          (ensures
             (index (insert s i a) i = a
             /\ (forall j. 0 <= j && j < i
@@ -92,18 +157,15 @@ module Tesseract.Specs.SeqExt
             /\ (forall j. i < j && j < length (insert s i a)
                ==> index (insert s i a) j = index s (j - 1))))
 
-   val remove:
-      s: seq 'a{length s > 0}
-      -> i: nat{i < length s}
-      -> 'a
-      -> Tot (seq 'a)
-
    val lemma_remove__length:
       s: seq 'a{length s > 0}
       -> i: nat{i < length s}
       -> a: 'a
       -> Lemma
-         (requires True)
+         (requires (True))
+            // bug: if the parenthesis is dropped from the preceeding
+            // expression, f* will silently fail to build the definition if
+            // included as a dependency.
          (ensures (length (remove s i a) = length s - 1))
          [SMTPat (length (remove s i a))]
 
@@ -112,6 +174,10 @@ module Tesseract.Specs.SeqExt
       -> i: nat{i < length s}
       -> a: 'a
       -> Lemma
+         (requires (True))
+            // bug: if the parenthesis is dropped from the preceeding
+            // expression, f* will silently fail to build the definition if
+            // included as a dependency.
          (ensures
             ((forall j. 0 <= j && j < i
                ==> index (remove s i a) j = index s j)
