src/specs/seqext.fst
@@ -24,6 +24,71 @@
 module Tesseract.Specs.SeqExt
    open Seq
 
+   val __map__loop:
+      // mapping function
+      ('a -> Tot 'b)
+      // input sequence
+      -> s: seq 'a
+      // accumulator; in this case, the output sequence.
+      -> c: seq 'b{length c <= length s}
+      -> Tot (seq 'b)
+         (decreases (length s - length c))
+   let rec __map__loop f s c =
+      let i = length c in
+      if i < length s then
+         let a = index s i in
+         let c' = append c (create 1 (f a)) in
+         __map__loop f s c'
+      else
+         c
+
+   val __lemma_map__loop__length:
+      f: ('a -> Tot 'b)
+      -> s: seq 'a
+      -> c: seq 'b{length c <= length s}
+      -> Lemma
+         (requires (True))
+         (ensures (length (__map__loop f s c) = length s))
+         (decreases (length s - length c))
+   let rec __lemma_map__loop__length f s c =
+      let i = length c in
+      if i < length s then
+         let a = index s i in
+         let c' = append c (create 1 (f a)) in
+         __lemma_map__loop__length f s c'
+      else
+         ()
+
+   val __lemma_map__loop__map:
+      f: ('a -> Tot 'b)
+      -> s: seq 'a
+      -> c: seq 'b{length c <= length s}
+      -> Lemma
+         (requires ((forall i. 0 <= i && i < length c ==> index c i = f (index s i))))
+         (ensures
+            (forall i.
+               0 <= i
+               && i < length (__map__loop f s c)
+               ==>
+                  (i < length s
+                  && index (__map__loop f s c) i = f (index s i))))
+         (decreases (length s - length c))
+   let rec __lemma_map__loop__map f s c =
+      let i = length c in
+      if i < length s then
+         let a = index s i in
+         let c' = append c (create 1 (f a)) in
+         __lemma_map__loop__map f s c'
+      else
+         ()
+
+   let map f s =
+      __map__loop f s createEmpty
+   let lemma_map__length f s =
+      __lemma_map__loop__length f s createEmpty
+   let lemma_map__map f s i =
+      __lemma_map__loop__map f s createEmpty
+
    val __mem__loop:
       s: seq 'a
       -> i: nat{i < length s}
@@ -47,7 +112,56 @@ module Tesseract.Specs.SeqExt
 
    let lemma_mem__mem s a = ()
 
-   val __filter_loop:
+   let lemma_mem__append s0 s1 =
+       admit ()
+
+   (* val __lemma_mem__index__loop:
+    s: seq 'a
+    -> i: nat{i < length s}
+    -> Lemma
+       (requires (forall j. 0 <= j && j < i ==> mem s (index s j)))
+       (ensures (forall j. 0 <= j && j <= i ==> mem s (index s j)))
+       (decreases (length s - i))
+    let rec __lemma_mem__index__loop s i =
+       let z = length s - 1 in
+       if z = i then
+          ()
+       else
+          __lemma_mem__index__loop s i *)
+
+   val __lemma_mem__index__loop:
+   s: seq 'a{length s > 0}
+   -> i: nat{i < length s}
+   -> a: 'a{a = index s i}
+   -> j: nat{j < length s}
+   -> c: bool
+   -> Lemma
+      (requires (j > i ==> c))
+      (ensures (j >= i ==> __mem__loop s j a c))
+      (decreases (length s - j))
+   let rec __lemma_mem__index__loop s i a j c =
+      let z = length s - 1 in
+      let c' = c || (a = index s j) in
+      if z = j then
+         ()
+      else
+         __lemma_mem__index__loop s i a (j + 1) c'
+
+   // hypothesis: this lemma isn't working because __mem__loop needs to be unrolled completely in order to prove this.
+   // validated. limiting the length of the sequence and setting the fuel to be > length verifies the lemma.
+   // solution: use map to implement mem.
+#set-options "--initial_fuel 100 --max_fuel 100"
+   val lemma_mem__index:
+      s:seq 'a{length s > 0}
+      -> i:nat{i < length s}
+      -> Lemma
+         (requires (True))
+         (ensures (mem s (index s i)))
+         [SMTPat (index s i)]
+   let lemma_mem__index s i =
+      __lemma_mem__index__loop s i (index s i) 0 false
+
+   val __filter__loop:
       // predicate; if false, then the element is discarded from the sequence.
       ('a -> Tot bool)
       // input sequence
@@ -58,7 +172,7 @@ module Tesseract.Specs.SeqExt
       -> c: seq 'a
       -> Tot (seq 'a)
          (decreases (length s - i))
-   let rec __filter_loop p s i c =
+   let rec __filter__loop p s i c =
       let z = length s - 1 in
       let a = index s i in
       let c' =
@@ -69,24 +183,24 @@ module Tesseract.Specs.SeqExt
       if i = z then
          c'
       else
-         __filter_loop p s (i + 1) c'
+         __filter__loop p s (i + 1) c'
 
    let filter p s =
       if length s = 0 then
          createEmpty
       else
-         __filter_loop p s 0 createEmpty
+         __filter__loop p s 0 createEmpty
 
-   val __lemma_filter_loop__length:
+   val __lemma_filter__loop__length:
       p: ('a -> Tot bool) ->
       s: seq 'a{length s > 0} ->
       i: nat{i < length s} ->
       c: seq 'a ->
       Lemma
          (requires (length c <= i))
-         (ensures (length (__filter_loop p s i c) <= length s))
+         (ensures (length (__filter__loop p s i c) <= length s))
          (decreases (length s - i))
-   let rec __lemma_filter_loop__length p s i c =
+   let rec __lemma_filter__loop__length p s i c =
       let z = length s - 1 in
       let a = index s i in
       let c' =
@@ -97,13 +211,13 @@ module Tesseract.Specs.SeqExt
       if i = z then
          ()
       else
-         __lemma_filter_loop__length p s (i + 1) c'
+         __lemma_filter__loop__length p s (i + 1) c'
 
    let lemma_filter__length p s =
       if length s = 0 then
          ()
       else
-         __lemma_filter_loop__length p s 0 createEmpty
+         __lemma_filter__loop__length p s 0 createEmpty
 
    val __lemma_filter__loop__admission:
       p: ('a -> Tot bool)
@@ -114,8 +228,8 @@ module Tesseract.Specs.SeqExt
       -> Lemma
          (requires (forall j. 0 <= j && j < length c ==> p (index c j)))
          (ensures
-            (k < length (__filter_loop p s i c)
-            ==> p (index (__filter_loop p s i c) k)))
+            (k < length (__filter__loop p s i c)
+            ==> p (index (__filter__loop p s i c) k)))
          (decreases (length s - i))
    let rec __lemma_filter__loop__admission p s i c k =
       let z = length s - 1 in
@@ -135,6 +249,48 @@ module Tesseract.Specs.SeqExt
          ()
       else
          __lemma_filter__loop__admission p s 0 createEmpty k
+
+   val __lemma_filter__loop__mem:
+      p: ('a -> Tot bool)
+      -> s: seq 'a{length s > 0}
+      -> i: nat{i < length s}
+      -> c: seq 'a
+      -> Lemma
+         (requires
+            (forall j.
+               (0 <= j && j < length c) ==> (mem s (index c j))))
+         (ensures
+            (forall j.
+               (0 <= j && j < length (__filter__loop p s i c)) ==> (mem s (index (__filter__loop p s i c) j))))
+         (decreases (length s - i))
+   let rec __lemma_filter__loop__mem p s i c =
+      let z = length s - 1 in
+      let a = index s i in
+      //lemma_mem__mem s a;
+      let c' =
+         if p a then
+            append c (create 1 a)
+         else
+            c in
+      if i = z then
+         ()
+      else
+         admit ()//__lemma_filter__loop__mem p s (i + 1) c'
+
+   (*val lemma_filter__mem:
+      p: ('a -> Tot bool) ->
+      s: seq 'a ->
+      Lemma
+         (requires (True))
+         (ensures
+            (forall i.
+               0 <= i && i < length (filter p s)
+               ==> mem s (index (filter p s) i)))
+   let lemma_filter__mem p s =
+      if length s = 0 then
+         ()
+      else
+         __lemma_filter__loop__mem p s 0 createEmpty *)
 
    let insert s i a =
       let l = slice s 0 i in
